Pullback/SSA/VarMap.lean
@@ -2,50 +2,57 @@ import Pullback.SSA.Basic
 
 open Lean
 
-theorem VarMap.get_eq_some_imp_any (vars : VarMap) (key : Name) (a : SSAType) : vars.get key = some a → vars.any (·.1 = key) := by
-    simp [Array.get, Array.findLast?, Array.find?_eq_some_iff_getElem]
+variable {α β} [DecidableEq α]
+
+theorem Map.get_eq_some_imp_any (vars : Map α β) (key : α) (a : β) :
+        vars.get key = some a → vars.any (·.1 = key) := by
+    simp [Map.get, Array.findLast?, Array.find?_eq_some_iff_getElem]
     grind
 
-theorem VarMap.get_isSome_iff_any (vars : VarMap) (key : Name) : (vars.get key).isSome ↔ vars.any (·.1 = key) := sorry
+theorem Map.get_isSome_iff_any (vars : Map α β) (key : α) :
+    (vars.get key).isSome ↔ vars.any (·.1 = key) := sorry
 
-theorem VarMap.get_mem (vars : VarMap) (name : Name) (type : SSAType) : (name, type) ∈ vars → ∃ a, vars.get name = some a := by
+theorem Map.get_mem {α β} [DecidableEq α] (vars : Map α β) (key : α) (val : β) :
+        (key, val) ∈ vars → ∃ a, vars.get key = some a := by
     intro h
-    have := VarMap.get_isSome_iff_any
+    have := Map.get_isSome_iff_any (α := α) (β := β)
     simp only [Option.isSome_iff_exists] at this
     simp only [this, Array.any_eq_true, decide_eq_true_eq]
     simp only [Array.mem_iff_getElem] at h
     grind
 
 
-theorem VarMap.mem_get (vars: VarMap) (name : Name) (type : SSAType) : vars.get name = some type → (name, type) ∈ vars := sorry
+theorem Map.mem_get (vars: Map α β) (key : α) (val : β) :
+    vars.get key = some val → (key, val) ∈ vars := sorry
 
-theorem VarMap.get_push (vars : VarMap) (last : Name × SSAType) (key : Name) : ((vars.push last)).get key = if last.1 = key then some last.2 else vars.get key := sorry
+theorem Map.get_push (vars : Map α β) (last : α × β) (key : α) :
+    Map.get (vars.push last) key = if last.1 = key then some last.2 else vars.get key := sorry
 
 
-theorem VarMap.get_eq_none_iff_not_any (vars : VarMap) (key : Name) : vars.get key = none ↔ ¬ vars.any (·.1 = key) := sorry
+theorem Map.get_eq_none_iff_not_any (vars : Map α β) (key : α) : vars.get key = none ↔ ¬ vars.any (·.1 = key) := sorry
 
 /- two VarMaps are equivalent if the non shadowed variables agree on types at all names, and the set of unshadowed names is the same -/
-def VarMap.equiv (vars₁ vars₂ : VarMap) : Prop :=
+def Map.equiv (vars₁ vars₂ : Map α β) : Prop :=
     {name | vars₁.any (·.1 = name)} = {name | vars₂.any (·.1 = name)} ∧ ∀ name, vars₁.any (·.1 = name) → vars₁.get name = vars₂.get name
 
-def VarMap.equiv_symm {vars₁ vars₂ : VarMap} : vars₁.equiv vars₂ → vars₂.equiv vars₁ := by
+def Map.equiv_symm {vars₁ vars₂ : Map α β} : vars₁.equiv vars₂ → vars₂.equiv vars₁ := by
     simp only [equiv, Array.any_eq_true', decide_eq_true_eq, forall_exists_index, and_imp]
     intro h1 h2
-    have : ∀ (name : Name) (x : Name × SSAType), x ∈ vars₂ → x.1 = name → Array.get vars₂ name = Array.get vars₁ name := by
+    have : ∀ (name : α) (x : α × β), x ∈ vars₂ → x.1 = name → Map.get vars₂ name = Map.get vars₁ name := by
         intro name a ha1 ha2
         rw [Set.ext_iff] at h1
         specialize h1 a.1
         grind
     tauto
 
-def VarMap.equiv_push (vars₁ vars₂ : VarMap) (hvars : vars₁.equiv vars₂) (varname : Name) (vartype : SSAType) : VarMap.equiv (vars₁.push (varname, vartype)) (vars₂.push (varname, vartype)) := by
+def Map.equiv_push (vars₁ vars₂ : Map α β) (hvars : vars₁.equiv vars₂) (varname : α) (vartype : β) : Map.equiv (vars₁.push (varname, vartype)) (vars₂.push (varname, vartype)) := by
     simp only [equiv, Array.any_eq_true, decide_eq_true_eq, forall_exists_index, Array.size_push, Array.any_push', Bool.or_eq_true] at ⊢ hvars
     apply And.intro
     · ext name
       rw [Set.ext_iff] at hvars
       grind only [usr Set.mem_setOf_eq]
     · intro name H
-      have := VarMap.get_push
+      have := Map.get_push (α := α) (β := β)
       simp only [Prod.forall] at this
       rw [this]
       cases em (varname = name) with
@@ -59,7 +66,7 @@ def VarMap.equiv_push (vars₁ vars₂ : VarMap) (hvars : vars₁.equiv vars₂)
         simp [hr]
         grind only
 
-def VarMap.equiv_push_of_shadow (vars : VarMap) (varname : Name) (vartype : SSAType) (hvar_type : vars.get varname = some vartype): VarMap.equiv vars (vars.push (varname, vartype)) := sorry
+def Map.equiv_push_of_shadow (vars : Map α β) (varname : α) (vartype : β) (hvar_type : vars.get varname = some vartype): Map.equiv vars (vars.push (varname, vartype)) := sorry
 
 theorem SSAExpr.inferType_eq_of_vars_equiv (vars₁ vars₂ : VarMap) (hvars : vars₁.equiv vars₂) : (expr : SSAExpr) → expr.inferType vars₁ = expr.inferType vars₂
 | const c => by simp only [inferType]
@@ -68,38 +75,37 @@ theorem SSAExpr.inferType_eq_of_vars_equiv (vars₁ vars₂ : VarMap) (hvars : v
     rw [inferType_eq_of_vars_equiv vars₁ vars₂ hvars val]
     congr
     ext valType a
-    have := inferType_eq_of_vars_equiv (vars₁.push (varname, valType)) (vars₂.push (varname, valType)) (VarMap.equiv_push vars₁ vars₂ hvars varname valType) body
+    have := inferType_eq_of_vars_equiv (vars₁.push (varname, valType)) (vars₂.push (varname, valType)) (Map.equiv_push vars₁ vars₂ hvars varname valType) body
     grind only
 | lam varname type body => by
     simp only [inferType]
-    have := inferType_eq_of_vars_equiv (vars₁.push (varname, type)) (vars₂.push (varname, type)) (VarMap.equiv_push vars₁ vars₂ hvars varname type) body
+    have := inferType_eq_of_vars_equiv (vars₁.push (varname, type)) (vars₂.push (varname, type)) (Map.equiv_push vars₁ vars₂ hvars varname type) body
     grind only
 | app f x => by
     simp only [inferType]
     rw [inferType_eq_of_vars_equiv vars₁ vars₂ hvars f, inferType_eq_of_vars_equiv vars₁ vars₂ hvars x]
 | var name => by
     simp only [inferType]
-    simp only [VarMap.equiv] at hvars
+    simp only [Map.equiv] at hvars
     match h : vars₁.get name with
     | some type =>
         have h' := h
-        apply VarMap.get_eq_some_imp_any at h
+        apply Map.get_eq_some_imp_any at h
         have := hvars.2 name (by grind)
         grind
     | none =>
         have h' := h
-        rw [VarMap.get_eq_none_iff_not_any] at h
+        rw [Map.get_eq_none_iff_not_any] at h
         have := hvars.1
         rw [Set.ext_iff] at this
         specialize this name
         simp only [Array.any_eq_true, decide_eq_true_eq, Set.mem_setOf_eq] at this
-        grind only [Array.any_eq_true, VarMap.get_eq_none_iff_not_any]
+        grind only [Array.any_eq_true, Map.get_eq_none_iff_not_any]
 
-def VarMap.submap (vars₁ vars₂ : VarMap) : Prop :=
+def Map.submap (vars₁ vars₂ : Map α β) : Prop :=
     {name | vars₁.any (·.1 = name)} ⊆ {name | vars₂.any (·.1 = name)} ∧ ∀ name, vars₁.any (·.1 = name) → vars₁.get name = vars₂.get name
 
-def VarMap.submap_push (vars₁ vars₂ : VarMap) (hvars : vars₁.submap vars₂) (varname : Name) (vartype : SSAType) : (cast (β := VarMap) rfl (vars₁.push (varname, vartype))).submap (vars₂.push (varname, vartype)) := by
-    simp only [cast_eq]
+def Map.submap_push (vars₁ vars₂ : Map α β) (hvars : vars₁.submap vars₂) (varname : α) (vartype : β) : Map.submap (vars₁.push (varname, vartype)) (vars₂.push (varname, vartype)) := by
     simp only [submap, Array.any_eq_true, decide_eq_true_eq, forall_exists_index, Array.size_push, Array.any_push', Bool.or_eq_true] at ⊢ hvars
     apply And.intro
     · intro name
@@ -113,7 +119,7 @@ def VarMap.submap_push (vars₁ vars₂ : VarMap) (hvars : vars₁.submap vars�
       | inr hr =>
         grind
     · intro name hName
-      have := VarMap.get_push
+      have := Map.get_push (α := α) (β := β)
       simp at this
       simp [this]
       cases em (varname = name) with
@@ -123,16 +129,16 @@ def VarMap.submap_push (vars₁ vars₂ : VarMap) (hvars : vars₁.submap vars�
         simp only [hr, or_false, ↓reduceIte] at ⊢ hName
         grind
 
-theorem VarMap.push_valid {var : Name} {varT : SSAType} {mutVars vars : VarMap} (hvarT : Array.get mutVars var = some varT) (hMut₂ : ∀ x ∈ mutVars, vars.get x.1 = some x.2) : ∀ (x : Name × SSAType), x ∈ mutVars → (Array.push vars (var, varT)).get x.1 = some x.2 := by
-    simp [VarMap.get_push]
-    have : Array.get mutVars var = Array.get vars var := by
-        have := VarMap.mem_get mutVars var varT hvarT
+theorem Map.push_valid {var : α} {varT : β} {mutVars vars : Map α β} (hvarT : Map.get mutVars var = some varT) (hMut₂ : ∀ x ∈ mutVars, vars.get x.1 = some x.2) : ∀ (x : α × β), x ∈ mutVars → Map.get (Array.push vars (var, varT)) x.1 = some x.2 := by
+    simp [Map.get_push]
+    have : Map.get mutVars var = Map.get vars var := by
+        have := Map.mem_get mutVars var varT hvarT
         specialize hMut₂ _ this
         grind
-    have : Array.get vars var = varT := by grind
+    have : Map.get vars var = varT := by grind
     grind
 
-theorem SSAExpr.inferType!_eq_of_vars_equiv {vars₁ vars₂ : VarMap} (hvars : VarMap.equiv vars₁ vars₂) {expr : SSAExpr} :
+theorem SSAExpr.inferType!_eq_of_vars_equiv {vars₁ vars₂ : VarMap} (hvars : Map.equiv vars₁ vars₂) {expr : SSAExpr} :
     expr.inferType! vars₁ = expr.inferType! vars₂ := sorry
 
-#check mkMutTuple
+def ArgMap.submapVars (args : ArgMap) (vars : VarMap) : Prop := Map.submap (args.map (fun (name, x) => (name, x.inferType))) vars
